code/bignum/Hacl.Impl.Exponentiation.fsti
@@ -88,7 +88,7 @@ let lsqr_st
 
 
 inline_for_extraction noextract
-class lexp (a_t:inttype_a) (len:size_t{v len > 0}) (ctx_len:size_t) = {
+class concrete_ops (a_t:inttype_a) (len:size_t{v len > 0}) (ctx_len:size_t) = {
   to: Ghost.erased (to_comm_monoid a_t len ctx_len);
   //lone: lone_st a_t len ctx_len to;
   lmul: lmul_st a_t len ctx_len to;
@@ -97,11 +97,11 @@ class lexp (a_t:inttype_a) (len:size_t{v len > 0}) (ctx_len:size_t) = {
 
 
 inline_for_extraction noextract
-val lexp_rl:
+val lexp_rl_vartime:
     #a_t:inttype_a
   -> len:size_t{v len > 0}
   -> ctx_len:size_t
-  -> k:lexp a_t len ctx_len
+  -> k:concrete_ops a_t len ctx_len
   -> ctx:lbuffer (uint_t a_t SEC) ctx_len
   -> a:lbuffer (uint_t a_t SEC) len
   -> bLen:size_t
@@ -124,11 +124,11 @@ val lexp_rl:
 
 
 inline_for_extraction noextract
-val lexp_mont_ladder_swap:
+val lexp_mont_ladder_swap_consttime:
     #a_t:inttype_a
   -> len:size_t{v len > 0}
   -> ctx_len:size_t
-  -> k:lexp a_t len ctx_len
+  -> k:concrete_ops a_t len ctx_len
   -> ctx:lbuffer (uint_t a_t SEC) ctx_len
   -> a:lbuffer (uint_t a_t SEC) len
   -> bLen:size_t
@@ -155,7 +155,7 @@ val lexp_pow_in_place:
     #a_t:inttype_a
   -> len:size_t{v len > 0}
   -> ctx_len:size_t
-  -> k:lexp a_t len ctx_len
+  -> k:concrete_ops a_t len ctx_len
   -> ctx:lbuffer (uint_t a_t SEC) ctx_len
   -> acc:lbuffer (uint_t a_t SEC) len
   -> b:size_t ->
@@ -168,7 +168,7 @@ val lexp_pow_in_place:
 
 
 inline_for_extraction noextract
-let lexp_fw_st (a_t:inttype_a) (len:size_t{v len > 0}) (ctx_len:size_t) (k:lexp a_t len ctx_len) =
+let lexp_fw_st (a_t:inttype_a) (len:size_t{v len > 0}) (ctx_len:size_t) (k:concrete_ops a_t len ctx_len) =
     ctx:lbuffer (uint_t a_t SEC) ctx_len
   -> a:lbuffer (uint_t a_t SEC) len
   -> bLen:size_t
@@ -196,7 +196,7 @@ val lexp_fw_vartime:
     #a_t:inttype_a
   -> len:size_t{v len > 0}
   -> ctx_len:size_t
-  -> k:lexp a_t len ctx_len ->
+  -> k:concrete_ops a_t len ctx_len ->
   lexp_fw_st a_t len ctx_len k
 
 
@@ -205,53 +205,5 @@ val lexp_fw_consttime:
     #a_t:inttype_a
   -> len:size_t{v len > 0}
   -> ctx_len:size_t
-  -> k:lexp a_t len ctx_len ->
+  -> k:concrete_ops a_t len ctx_len ->
   lexp_fw_st a_t len ctx_len k
-
-
-inline_for_extraction noextract
-let lexp_double_fw_st (a_t:inttype_a) (len:size_t{v len > 0}) (ctx_len:size_t) (k:lexp a_t len ctx_len) =
-    ctx:lbuffer (uint_t a_t SEC) ctx_len
-  -> a1:lbuffer (uint_t a_t SEC) len
-  -> bLen:size_t
-  -> bBits:size_t{0 < v bBits /\ (v bBits - 1) / bits a_t < v bLen}
-  -> b1:lbuffer (uint_t a_t SEC) bLen
-  -> a2:lbuffer (uint_t a_t SEC) len
-  -> b2:lbuffer (uint_t a_t SEC) bLen
-  -> acc:lbuffer (uint_t a_t SEC) len
-  -> l:size_t{0 < v l /\ v l < bits a_t /\ pow2 (v l) * v len <= max_size_t /\ v l < 32} ->
-  Stack unit
-  (requires fun h ->
-    live h a1 /\ live h b1 /\ live h a2 /\ live h b2 /\ live h acc /\ live h ctx /\
-    eq_or_disjoint a1 a2 /\ disjoint a1 acc /\ disjoint a1 ctx /\
-    disjoint a2 acc /\ disjoint a2 ctx /\
-    disjoint acc b1 /\ disjoint acc b2 /\ disjoint acc ctx /\
-    BD.bn_v h b1 < pow2 (v bBits) /\
-    BD.bn_v h b2 < pow2 (v bBits) /\
-    k.to.linv_ctx (as_seq h ctx) /\
-    k.to.linv (as_seq h a1) /\ k.to.linv (as_seq h a2) /\
-    k.to.linv (as_seq h acc) /\ k.to.refl (as_seq h acc) == k.to.comm_monoid.S.one)
-  (ensures  fun h0 _ h1 -> modifies (loc acc) h0 h1 /\
-    k.to.linv (as_seq h1 acc) /\
-    k.to.refl (as_seq h1 acc) ==
-    S.exp_double_fw #k.to.a_spec k.to.comm_monoid
-      (k.to.refl (as_seq h0 a1)) (v bBits) (BD.bn_v h0 b1)
-      (k.to.refl (as_seq h0 a2)) (BD.bn_v h0 b2) (v l))
-
-
-inline_for_extraction noextract
-val lexp_double_fw_vartime:
-    #a_t:inttype_a
-  -> len:size_t{v len > 0}
-  -> ctx_len:size_t
-  -> k:lexp a_t len ctx_len ->
-  lexp_double_fw_st a_t len ctx_len k
-
-
-inline_for_extraction noextract
-val lexp_double_fw_consttime:
-    #a_t:inttype_a
-  -> len:size_t{v len > 0}
-  -> ctx_len:size_t
-  -> k:lexp a_t len ctx_len ->
-  lexp_double_fw_st a_t len ctx_len k
